WIP

proofmode/HTactics2.v
@@ -41,7 +41,7 @@ Section MODE.
 
   Context `{Σ: GRA.t}.
 
-  Definition OwnT := Own.
+  Let OwnT := Own.
 
   Local Transparent HoareFun HoareFunArg HoareFunRet HoareCall.
 
@@ -125,7 +125,7 @@ Section MODE.
                               (bupd (P_tgt mn x_tgt arg_tgt arg_tgt ** FR))>>
                    /\
             <<SIM: forall mr_src' fr_src fr_tgt
-                  (ACC: current_iPropL (fr_src ⋅ mr_src' ⋅ mr_tgt)
+                  (ACC: current_iPropL (fr_src ⋅ (mr_tgt ⋅ mr_src'))
                                        [("FR", FR); ("TF", OwnT fr_tgt); ("TM", OwnT mr_tgt)]),
                 gpaco8 (_sim_itree (mk_wf R) le) (cpn8 (_sim_itree (mk_wf R) le)) r rg _ _ eqr true true a
                        (Any.pair mp_src (mr_tgt ⋅ mr_src')↑, k_src (fr_src, ((mn, x_src), arg_src)))
@@ -174,6 +174,15 @@ Section MODE.
       iStopProof. eapply from_semantic; et.
     }
     mUpd "A". mDesAll. mRename "A1" into "TM". mRename "A2" into "TF". mRename "A" into "FR". ss.
+    replace (fr_src ⋅ (mr_tgt ⋅ mr_src')) with (fr_src ⋅ mr_src' ⋅ mr_tgt) by r_solve. ss.
+  Qed.
+
+  (*** TODO: update the one in IPM.v ***)
+  Lemma from_semantic (a: Σ) (P: iProp') (SAT: P a)
+    :
+      bi_entails (Own a) (P).
+  Proof.
+    uipropall. ss. i. eapply iProp_mono; et.
   Qed.
 
   Lemma hcall_clo2
@@ -202,18 +211,16 @@ Section MODE.
                (tbr = true -> is_pure (fsp_src.(measure) x_src)) /\
                  (tbr = false -> (fsp_src.(measure) x_src) = ord_top))
 
-        (POST: forall (ret_tgt: Any.t) (mr_src1 mr_tgt1: Σ) (mp_src1 mp_tgt1 : Any.t) a1
-                      (ret_src: Any.t)
-                      (WLE: le a0 a1)
-                      fr_src1 fr_tgt1 x_tgt,
+        (POST: forall (ret_src ret_tgt: Any.t) (mp_src1 mp_tgt1 : Any.t) a1 (WLE: le a0 a1) x_tgt,
             exists J,
-              (<<UPDATABLE: bi_entails (FR ** OwnT fr_tgt1 ** OwnT mr_tgt1 ** R a1 mp_src1 mp_tgt1 **
+              (<<UPDATABLE: bi_entails (FR ** R a1 mp_src1 mp_tgt1 **
                                           fsp_src.(postcond) (Some mn) x_src ret_src ret_tgt)
-                                      (OwnT fr_tgt1 ** OwnT mr_tgt1 **
-                                            fsp_tgt.(postcond) (Some mn) x_tgt ret_src ret_tgt ** J)>>) /\
-                <<SIM: forall (ACC: current_iPropL (fr_src1 ⋅ mr_src1) [("J", J)]),
+                                      (fsp_tgt.(postcond) (Some mn) x_tgt ret_src ret_tgt ** J)>>) /\
+                <<SIM: forall fr_src1 fr_tgt1 mr_src1 mr_tgt1
+                              (ACC: current_iPropL (fr_src1 ⋅ (mr_tgt1 ⋅ mr_src1))
+                                                   [("J", J); ("TF", OwnT fr_tgt1); ("TM", OwnT mr_tgt1)]),
                 gpaco8 (_sim_itree (mk_wf R) le) (cpn8 (_sim_itree (mk_wf R) le)) rg rg _ _ eqr true true a
-                       (Any.pair mp_src1 (mr_src1 ⋅ mr_tgt1)↑, k_src (fr_src1, ret_src))
+                       (Any.pair mp_src1 (mr_tgt1 ⋅ mr_src1)↑, k_src (fr_src1, ret_src))
                        (Any.pair mp_tgt1 mr_tgt1↑, k_tgt (fr_tgt1, ret_tgt))>>)
     :
       gpaco8 (_sim_itree (mk_wf R) le) (cpn8 (_sim_itree (mk_wf R) le)) r rg _ _ eqr m n a
@@ -238,9 +245,8 @@ Section MODE.
     { iDestruct "H" as "[[A B] C]". instantiate (1:=_ ** _ ** _).
       iSplitR "A"; try iAssumption. iSplitR "B"; try iAssumption. }
     mDesAll.
-    mAssert (#=> _) with "A1".
-    { iStopProof. eapply from_semantic. eauto. }
-    mUpd "A3".
+    mAssert (_) with "A1".
+    { iStopProof. eapply from_semantic; eauto. }
     mAssert (#=> _) with "A A3".
     { assert(x1 = arg_tgt).
       { admit "simple". }
@@ -270,249 +276,115 @@ Section MODE.
     rename x7 into ret_src. rename vret into ret_tgt.
     inv WF. rewrite Any.pair_split in *. clarify. rewrite Any.upcast_downcast in *. clarify.
     move POST at bottom.
-    specialize (POST ret_tgt mr_src' mr_tgt mp_src2 mp_tgt w1 ret_src WLE fr_src fr_tgt x_tgt). des.
-    assert(ACC:=current_iPropL_init "A" x6).
-    mAssert (_ ∗ _ ∗ _ ∗ _ ∗ _)%I with "A".
-    { iDestruct "A" as "[[A [B C]] [D E]]".
-      iSplitL "A"; try iAssumption. iSplitL "B"; try iAssumption.
-      iSplitL "C"; try iAssumption. iSplitL "D"; try iAssumption. }
+    specialize (POST ret_src ret_tgt mp_src2 mp_tgt w1 WLE x_tgt). des.
+    assert(T: URA.wf (ri_src ⋅ fr_src ⋅ mr_src')).
+    { eapply URA.wf_mon; et. instantiate (1:= fr_tgt ⋅ mr_tgt). r_wf x6. }
+    assert(ACC:=current_iPropL_init "A" T).
+    mAssert (_ ∗ _ ∗ _)%I with "A".
+    { iDestruct "A" as "[[A B] C]". iSplitL "A"; try iAssumption. iSplitL "B"; try iAssumption. }
     mDesAll.
-    mAssert (#=> _) with "A1".
+    mAssert (_) with "A".
     { iStopProof. eapply from_semantic; et. }
-    mAssert (#=> _) with "A".
+    mAssert (_) with "A1".
     { iStopProof. eapply from_semantic; et. }
-    mAssert (#=> _) with "A4".
+    mAssert (_) with "A2".
     { iStopProof. eapply from_semantic; et. eapply RSRC; et. eapply URA.wf_mon.
       instantiate (1:=ri_src ⋅ fr_src ⋅ fr_tgt ⋅ mr_tgt). r_wf x6.
     }
-    mUpd "A". mUpd "A5". mUpd "A1".
     eapply current_iProp_entail in ACC; cycle 1.
-    { etrans; try eassumption. iIntros "H". iDestruct "H" as "[A [B [C [D [E _]]]]]". iFrame. }
+    { etrans; try eassumption. iIntros "H". iDestruct "H" as "[A [B [C _]]]". iFrame. }
     inv ACC. rr in IPROP. repeat (autorewrite with iprop in IPROP; autounfold with iprop in IPROP; ss).
     des. subst.
-    clears fr_tgt_; clear fr_tgt_. rename a3 into fr_tgt_.
-    clears mr_tgt_; clear mr_tgt_. rename b1 into mr_tgt_.
-    rename b0 into ri_tgt. rename b into jr.
+    rename a1 into ri_tgt. rename b into jr.
+    assert(WF: URA.wf (ri_tgt ⋅ jr ⋅ (fr_tgt ⋅ mr_tgt))).
+    { eapply URA.updatable_wf; try apply x6.
+      replace (ri_src ⋅ (fr_src ⋅ fr_tgt) ⋅ (mr_tgt ⋅ mr_src')) with
+        ((fr_tgt ⋅ mr_tgt) ⋅ (ri_src ⋅ fr_src ⋅ mr_src')) by r_solve.
+      replace (ri_tgt ⋅ jr ⋅ (fr_tgt ⋅ mr_tgt)) with ((fr_tgt ⋅ mr_tgt) ⋅ (ri_tgt ⋅ jr)) by r_solve.
+      eapply URA.updatable_add; et; try refl. }
     repeat (ired_both; apply sim_itreeC_spec; econs). exists ri_tgt.
     repeat (ired_both; apply sim_itreeC_spec; econs). unshelve esplits; et.
-    { eapply URA.updatable_wf; et. etrans; et. rr in IPROP10. rr in IPROP11.
-      autorewrite with iprop in *. rr in IPROP10. rr in IPROP11. des; subst.
-      eapply URA.extends_updatable. exists (jr ⋅ ctx ⋅ ctx0). r_solve. }
+    { eapply URA.wf_mon. instantiate (1:=jr). r_wf WF. }
     steps.
-    repeat (ired_both; apply sim_itreeC_spec; econs). esplits; et.
+    repeat (ired_both; apply sim_itreeC_spec; econs). exists ret_tgt.
     repeat (ired_both; apply sim_itreeC_spec; econs). unshelve esplits; et.
+    { admit "simple". }
     steps.
-    TTTTTTTTTTTTTTTTTTT
     eapply SIM.
-    repeat (ired_both; apply sim_itreeC_spec; econs). unshelve esplits; et.
-    
-      et. }
-    mDesAll.
-    assert(ACC: current_iPropL [("I", ((((FR ** OwnT fr_tgt) ** OwnT mr_tgt) ** R w1 mp_src2 mp_tgt) **
-                postcond fsp_src (Some mn) x_src ret_src ret_tgt))]).
-    ss.
-    exploit POST; et. i; des.
-    repeat (ired_both; apply sim_itreeC_spec; econs). econs; et.
-    { econs; et. }
-    {
-      eapply URA.updatabe_add; et.
+    econs; et; cycle 1.
+    { replace (ri_src ⋅ (fr_src ⋅ fr_tgt) ⋅ (mr_tgt ⋅ mr_src'))
+        with ((ri_src ⋅ fr_src ⋅ mr_src') ⋅ (fr_tgt ⋅ mr_tgt)) by r_solve.
+      eapply URA.updatable_add; et. refl. }
+    { eapply to_semantic; cycle 1.
+      { r_wf WF. }
+      iIntros "[[A B] [C D]]". iSplitL "B".
+      { iStopProof. eapply from_semantic; et. }
+      iFrame. iSplitL "A"; iFrame.
+    }
+  Qed.
+
+  Lemma hret_clo2
+        A
+        mn r rg n m mp_src mp_tgt (mr_src mr_tgt: Σ) a0
+        Xs (Qs: option mname -> Xs -> Any.t -> Any.t -> iProp)
+        Xt (Qt: option mname -> Xt -> Any.t -> Any.t -> iProp)
+        xs xt vret_src vret_tgt
+        (le: A -> A -> Prop)
+        (eqr: Any.t -> Any.t -> Any.t -> Any.t -> Prop)
+        (R: A -> Any.t -> Any.t -> iProp)
+
+        fr_src fr_tgt
+
+        I
+        (ACC: current_iPropL (fr_src ⋅ (mr_tgt ⋅ mr_src)) [("I", I)])
+        (UPDATABLE:
+          bi_entails I (OwnT (fr_tgt) ** OwnT (mr_tgt) **
+                             (Qt mn xt vret_tgt vret_tgt
+                                 ==∗ ((∃ a, R a mp_src mp_tgt ** ⌜le a0 a⌝)
+                                        ** (Qs mn xs vret_src vret_tgt: iProp)))))
+        (EQ: forall mr_src mr_tgt a (WLE: le a0 a)
+                    (WF: mk_wf R a ((Any.pair mp_src mr_src), (Any.pair mp_tgt mr_tgt))),
+            eqr (Any.pair mp_src mr_src) (Any.pair mp_tgt mr_tgt) vret_tgt vret_tgt)
+    :
+      gpaco8 (_sim_itree (mk_wf R) le) (cpn8 (_sim_itree (mk_wf R) le)) r rg _ _ eqr m n a0
+             (Any.pair mp_src (mr_tgt ⋅ mr_src)↑, (HoareFunRet Qs mn xs (fr_src, vret_src)))
+             (Any.pair mp_tgt mr_tgt↑, (HoareFunRet Qt mn xt (fr_tgt, vret_tgt)))
+  .
+  Proof.
+    subst. unfold HoareFunRet, mput, mget, guarantee.
     steps.
-
-
-    eauto.
-    mDestruct (Own_Upd with "H") as "H".
-    assert (exists mr_src1 ro_src fr_src1,
-               (<<UPDATABLE: URA.updatable (fr_src0 ⋅ mr_src0 ⋅ mr_tgt0)
-                                           (mr_tgt1 ⋅ mr_src1 ⋅ ro_src ⋅ fr_src1)>>) /\
-               (<<RSRC: R a0 mp_src0 mp_tgt0 mr_src1>>) /\
-               (<<FRS: FR fr_src1>>) /\
-               (<<PRE: fsp_src.(precond) (Some mn) x_src arg_src arg_tgt ro_src>>)
-           ).
-    { clear - ACC UPDATABLE x x1 x2 x3.
-      eapply current_iPropL_pop in ACC; des.
-      eapply current_iPropL_pop in TL; des.
-      eapply current_iPropL_nil in TL0. ss.
-      specialize (UPDATABLE x0).
-      rr in HD0. autorewrite with iprop in HD0. des; clarify. r in HD1. autorewrite with iprop in HD1. des; clarify.
-      uipropall. exploit UPDATABLE; swap 1 2.
-      { esplits; et.
-        { rr in HD1. uipropall. eapply HD1; [|refl].
-          eapply wf_extends; try apply x.
-          exists (ro_tgt ⋅ fr_tgt ⋅ ctx0 ⋅ mr_tgt1). r_solve.
-        }
-        { rr. uipropall. }
-      }
-      { eapply wf_extends; et. r. exists (fr_tgt ⋅ ctx0 ⋅ mr_tgt1). instantiate (1:=ε). r_solve. }
-      { instantiate (1:= fr_tgt ⋅ ctx0 ⋅ mr_tgt1). r_wf x. }
-      i; des. clarify.
-      rr in x8. uipropall. des; ss.
-      esplits; et.
-      { eapply wf_extends; et. r. exists b. r_solve. }
-    }
-
-    unfold HoareCall at 1, mput, mget, assume, guarantee.
-    repeat (ired_both; apply sim_itreeC_spec; econs). eexists (_, _, _).
-    intro x_src.
-    ired_both. apply sim_itreeC_spec. econs.
-    hexploit (WEAKER x). i. des.
-    assert (exists mr_src0' rarg_src fr_src0',
-               (<<UPDATABLE: URA.updatable (fr0 ⋅ mr_src0) (mr_src0' ⋅ (rarg_src ⋅ fr_src0'))>>) /\
-               (<<RSRC: R a0 mp_src0 mp_tgt0 mr_src0'>>) /\
-               (<<FRS: FR fr_src0'>>) /\
-               (<<PRE: fsp0.(precond) (Some mn) x_tgt varg_src varg_tgt rarg_src>>)).
-    { inv ACC. uipropall.
-      hexploit UPDATABLE; try apply IPROP.
-      { eapply URA.updatable_wf; et. }
-      i. des. subst.
-      hexploit PRE; et. i. uipropall.
-      hexploit (H b); et.
-      { eapply URA.updatable_wf; et. etrans; et. etrans; et. eapply URA.extends_updatable.
-        exists (a2 ⋅ b0). r_solve. }
-      i; des.
-      esplits; et.
-      etrans; et. etrans; et.
-      replace (b0 ⋅ (r1 ⋅ a2)) with (b0 ⋅ a2 ⋅ r1) by r_solve.
-      eapply URA.updatable_add; et. rewrite URA.add_comm; ss.
-    }
-    des. exists (rarg_src, fr_src0', mr_src0').
-    repeat (ired_both; apply sim_itreeC_spec; econs). unshelve esplits.
-    { replace (rarg_src ⋅ fr_src0' ⋅ mr_src0') with (mr_src0' ⋅ (rarg_src ⋅ fr_src0')) by r_solve. ss. }
-    repeat (ired_both; apply sim_itreeC_spec; econs). exists x_tgt.
-    repeat (ired_both; apply sim_itreeC_spec; econs). exists varg_tgt.
-    repeat (ired_both; apply sim_itreeC_spec; econs). unshelve esplits; eauto.
-    repeat (ired_both; apply sim_itreeC_spec; econs). unshelve esplits; eauto.
-    { r in MEASURE. des_ifs; ss; des_ifs. eapply Ord.le_lt_lt; et. }
-    { i. spc PURE0. r in MEASURE. des_ifs; ss; des_ifs. }
-    { i. spc PURE1. r in MEASURE. des_ifs; ss; des_ifs. }
-    repeat (ired_both; apply sim_itreeC_spec; econs).
-    { econs; eauto. }
-    i. repeat (ired_both; apply sim_itreeC_spec; econs). i.
-    repeat (ired_both; apply sim_itreeC_spec; econs). inv WF.
-    repeat (ired_both; apply sim_itreeC_spec; econs). i.
-    repeat (ired_both; apply sim_itreeC_spec; econs). i.
-    repeat (ired_both; apply sim_itreeC_spec; econs). i.
-    ired_both. eapply POST; eauto. hexploit POST0. i.
-    uipropall. hexploit (H x0).
-    { eapply URA.wf_extends; et. exists (fr_src0' ⋅ mr_src). r_solve. }
-    { eassumption. }
-    i; des. econs.
-    { cbn. esplits; et. eapply RSRC0; et. eapply URA.wf_extends; et. exists (fr_src0' ⋅ x0). r_solve. }
-    { ss. }
-    replace (fr_src0' ⋅ mr_src ⋅ r1) with (r1 ⋅ fr_src0' ⋅ mr_src) by r_solve.
-    rewrite <- ! URA.add_assoc.
-    eapply URA.updatable_add; et. refl.
-  Qed.
-
-  Lemma harg_clo
-        A Rn Invsn Invtn
-        mn r rg
-        X (P: option mname -> X -> Any.t -> Any.t -> iProp) varg
-        mp_src mp_tgt (mr_src mr_tgt: Σ) f_tgt k_src
-        a (le: A -> A -> Prop)
-        (R: A -> Any.t -> Any.t -> iProp)
-        (eqr: Any.t -> Any.t -> Any.t -> Any.t -> Prop)
-        (WF: mk_wf R a ((Any.pair mp_src mr_src↑), (Any.pair mp_tgt mr_tgt↑)))
-        m n
-        (ARG:
-           forall x varg_src ctx
-                  (ACC: current_iPropL ctx [(Rn, P mn x varg_src varg);
-                                           (Invsn, R a mp_src mp_tgt);
-                                           (Invtn, OwnT mr_tgt)]),
-             gpaco8 (_sim_itree (mk_wf R) le) (cpn8 (_sim_itree (mk_wf R) le)) r rg _ _ eqr true n a
-                    (Any.pair mp_src mr_src↑, k_src (ctx, ((mn, x), varg_src)))
-                    (Any.pair mp_tgt mr_tgt↑, f_tgt))
-    :
-      gpaco8 (_sim_itree (mk_wf R) le) (cpn8 (_sim_itree (mk_wf R) le)) r rg _ _ eqr m n a
-             ((Any.pair mp_src mr_src↑), (HoareFunArg P (mn, varg) >>= k_src))
-             ((Any.pair mp_tgt mr_tgt↑), f_tgt)
-  .
-  Proof.
-    inv WF.
-    unfold HoareFunArg, mput, mget, assume, guarantee.
-    repeat (ired_both; apply sim_itreeC_spec; econs). intro x.
-    repeat (ired_both; apply sim_itreeC_spec; econs). intro varg_src.
-    repeat (ired_both; apply sim_itreeC_spec; econs). intros (rarg_src, ctx).
-    repeat (ired_both; apply sim_itreeC_spec; econs).
-    repeat (ired_both; apply sim_itreeC_spec; econs). intro VALID.
-    repeat (ired_both; apply sim_itreeC_spec; econs). intro ord_cur.
-    repeat (ired_both; gstep; econs). i.
-    eapply Any.pair_inj in H2. des; clarify. eapply Any.upcast_inj in H0. des; clarify.
-    eapply Any.pair_inj in H1. des; clarify. eapply Any.upcast_inj in H0. des; clarify.
-    ired_both. eapply ARG; et.
-    red. econs.
-    { instantiate (1:=rarg_src ⋅ mr_src). r_wf VALID. }
-    { ss. red. rr.
-      autorewrite with iprop; ss. esplits; et.
-      assert(T: URA.wf mr_src).
-      { eapply URA.wf_mon. instantiate (1:=(ctx ⋅ rarg_src)). r_wf VALID. }
-      spc RSRC.
-      clear - RSRC T VALID. unfold OwnT in *.
-      uipropall. des. clarify. esplits; et.
-      { rewrite URA.unit_id; ss. }
-      { rr. uipropall. }
-    }
-    Unshelve. all: try exact 0.
-  Qed.
-
-  Definition Exactly (r0: Σ) (Xtra: iProp): iProp :=
-    (Own r0 ∧ (⌜Entails (Own r0) Xtra⌝))%I.
-  
-  Hint Unfold Exactly: iprop.
-
-  Lemma harg_clo_tgt
-        A Xn Xtra Rn Invtn mp_tgt mr_tgt
-        Invtn' Xn'
-        mn r rg
-        X (P: option mname -> X -> Any.t -> Any.t -> iProp) varg
-        mp_src (mr_src: Σ) f_src k_tgt
-        a (le: A -> A -> Prop)
-        (R: A -> Any.t -> Any.t -> iProp)
-        (eqr: Any.t -> Any.t -> Any.t -> Any.t -> Prop)
-        m n
-        ctx x varg_tgt
-        (ACC: current_iPropL ctx [(Rn, P mn x varg_tgt varg); (Invtn, OwnT mr_tgt); (Xn, Xtra)])
-        (ARG: forall
-            rx
-            (ACC: current_iPropL ctx [(Invtn', OwnT mr_tgt); (Xn', Exactly rx Xtra)]),
-            gpaco8 (_sim_itree (mk_wf R) le) (cpn8 (_sim_itree (mk_wf R) le)) r rg _ _ eqr m true a
-                   (Any.pair mp_src mr_src↑, f_src)
-                   (Any.pair mp_tgt mr_tgt↑, k_tgt (ctx ⋅ rx, ((mn, x), varg_tgt))))
-    :
-      gpaco8 (_sim_itree (mk_wf R) le) (cpn8 (_sim_itree (mk_wf R) le)) r rg _ _ eqr m n a
-             (Any.pair mp_src mr_src↑, f_src)
-             (Any.pair mp_tgt mr_tgt↑, (HoareFunArg P (mn, varg) >>= k_tgt))
-  .
-  Proof.
+    rename c0 into ro_tgt. rename c into mr_tgt0. rename c1 into residue.
+    eapply current_iPropL_entail with (Hn:="I") in ACC; et. ss. unfold alist_add in *. ss.
+    mDesAll.
+    mAssert (#=> (_ ∗ _ ∗ _)) with "I A1".
+    { iCombine "I A1" as "A". iDestruct (Own_Upd with "A") as "A"; eauto. iMod "A".
+      iDestruct "A" as "[[A B] C]". iSplitL "A"; eauto. iSplitL "B"; eauto. }
+    mUpd "A2". mDesAll.
+    mAssert _ with "A2".
+    { iStopProof. eapply from_semantic; eauto. }
+    assert(x = vret_tgt).
+    { admit "simple". }
     subst.
-    unfold HoareFunArg, mput, mget, assume, guarantee. des.
-    repeat (ired_both; apply sim_itreeC_spec; econs). exists x.
-    repeat (ired_both; apply sim_itreeC_spec; econs). exists varg_tgt.
-    eapply current_iPropL_pop in ACC. des.
-    eapply current_iPropL_pop in TL. des.
-    eapply current_iPropL_pop in TL0. des. ss. clear_fast.
-    eapply current_iPropL_nil in TL. rename hdr into rarg_src. rename hdr0 into rinv. rename hdr1 into rx.
-    repeat (ired_both; apply sim_itreeC_spec; econs). exists (rarg_src, (ctx ⋅ rx)).
+    mAssert (#=> _) with "A A4".
+    { iSpecialize ("A" with "A4"). iAssumption. }
+    mUpd "A2". mDesAll.
+    inv ACC. rr in IPROP. repeat (autorewrite with iprop in IPROP; autounfold with iprop in IPROP; ss).
+    des. subst.
+    rename a1 into mr_src0. rename a2 into ro_src. rename a3 into mr_tgt0_. rename a4 into residue_.
     repeat (ired_both; apply sim_itreeC_spec; econs). esplits.
-    { clear - TL HD0. rr in HD0. uipropall. rr in HD0. des; clarify.
-      eapply wf_extends; et. exists ctx0. r_solve. }
-    repeat (ired_both; apply sim_itreeC_spec; econs). eexists; et.
-    ired_both. eapply ARG.
-    eapply current_iPropL_push; et.
-    eapply current_iPropL_push; et.
-    { instantiate (1:=rx). eapply current_iPropL_nil; et.
-      eapply wf_extends; et. exists rarg_src. r_solve.
-    }
-    { cbn. rr. uipropall. splits; [refl|].
-      rr. uipropall. i. eapply iProp_mono; eauto.
-    }
-  Unshelve. all: try exact 0.
+    repeat (ired_both; apply sim_itreeC_spec; econs). eexists (ro_src, ε, mr_tgt0 ⋅ mr_src0).
+    repeat (ired_both; apply sim_itreeC_spec; econs). unshelve esplits.
+    { etrans; et. eapply URA.extends_updatable.
+      rr in IPROP4. des; subst. exists (ctx ⋅ b2 ⋅ residue_). rewrite URA.unit_id. r_solve. }
+    repeat (ired_both; apply sim_itreeC_spec; econs). unshelve esplits; eauto.
+    steps. eapply EQ; et. econs; et.
   Qed.
 
-  Lemma current_iPropL_entail_all Hn ctx (l: iPropL) (P: iProp)
-        (ACC: current_iPropL ctx l)
+  Lemma current_iPropL_entail_all Hn fmr (l: iPropL) (P: iProp)
+        (ACC: current_iPropL fmr l)
         (ENTAIL: from_iPropL l -∗ (bupd P))
     :
-      current_iPropL ctx [(Hn, P)].
+      current_iPropL fmr [(Hn, P)].
   Proof.
     eapply current_iProp_upd.
     eapply current_iProp_entail; et.
@@ -543,432 +415,6 @@ Section MODE.
   (*   unfold from_iPropL at 2. etrans; et. (*** !!! ***) *)
   (* Qed. *)
 
-  Lemma harg_clo_tgt'
-        A Xn Invtn Xtra mp_tgt mr_tgt
-        mn r rg
-        X (P: option mname -> X -> Any.t -> Any.t -> iProp) varg
-        mp_src (mr_src: Σ) f_src k_tgt
-        a (le: A -> A -> Prop)
-        (R: A -> Any.t -> Any.t -> iProp)
-        (eqr: Any.t -> Any.t -> Any.t -> Any.t -> Prop)
-        m n
-        ctx x varg_tgt ips
-        (ACC: current_iPropL ctx ips)
-        (ENTAIL: bi_entails (from_iPropL ips) (bupd (P mn x varg_tgt varg ** OwnT mr_tgt ** Xtra)))
-        (ARG: forall
-            rx
-            (ACC: current_iPropL ctx [(Invtn, OwnT mr_tgt); (Xn, Exactly rx Xtra%I)]),
-            gpaco8 (_sim_itree (mk_wf R) le) (cpn8 (_sim_itree (mk_wf R) le)) r rg _ _ eqr m true a
-                   (Any.pair mp_src mr_src↑, f_src)
-                   (Any.pair mp_tgt mr_tgt↑, k_tgt (ctx ⋅ rx, ((mn, x), varg_tgt))))
-    :
-      gpaco8 (_sim_itree (mk_wf R) le) (cpn8 (_sim_itree (mk_wf R) le)) r rg _ _ eqr m n a
-             (Any.pair mp_src mr_src↑, f_src)
-             (Any.pair mp_tgt mr_tgt↑, (HoareFunArg P (mn, varg) >>= k_tgt))
-  .
-  Proof.
-    eapply current_iPropL_entail_all with (Hn:="A") in ACC; et.
-    mDesAll.
-    mAssert _ with "A1". { iAssumption. }
-    mAssert _ with "A2". { iAssumption. }
-    mAssert _ with "A". { iAssumption. }
-    eapply harg_clo_tgt; et.
-  Qed.
-
-  Lemma hret_clo_both
-        A (a: shelve__ A)
-        mn r rg n m mp_src mp_tgt (mr_src mr_tgt: Σ) a0
-        Xs (Qs: option mname -> Xs -> Any.t -> Any.t -> iProp)
-        Xt (Qt: option mname -> Xt -> Any.t -> Any.t -> iProp)
-        xs xt vret_src vret_tgt
-        (le: A -> A -> Prop)
-        (eqr: Any.t -> Any.t -> Any.t -> Any.t -> Prop)
-        (R: A -> Any.t -> Any.t -> iProp)
-
-        ctx rx
-        Invtn Xn Xtra
-        (ACC: current_iPropL ctx [(Invtn, OwnT mr_tgt); (Xn, Exactly rx Xtra)])
-
-        (WLE: le a0 a)
-
-        (UPDATABLE: forall vret_tgt_tgt,
-           bi_entails ((Qt mn xt vret_tgt vret_tgt_tgt: iProp) ** Xtra)
-                      (bupd (R a mp_src mp_tgt ** (Qs mn xs vret_src vret_tgt: iProp))))
-
-        (EQ: forall (mr_src1 mr_tgt1: Σ) (WLE: le a0 a) vret_tgt_tgt
-                    (WF: mk_wf R a (Any.pair mp_src mr_src1↑, Any.pair mp_tgt mr_tgt1↑)),
-                    bi_entails (Qt mn xt vret_tgt vret_tgt_tgt)
-            (⌜eqr (Any.pair mp_src mr_src1↑) (Any.pair mp_tgt mr_tgt1↑) vret_tgt vret_tgt_tgt⌝)%I)
-        (* (EQ: forall (mr_src1 mr_tgt1: Σ) (WLE: le a0 a) vret_tgt_tgt *)
-        (*             (QT: exists rq, Qt mn xt vret_tgt vret_tgt_tgt rq) *)
-        (*             (WF: mk_wf R a (Any.pair mp_src mr_src1↑, Any.pair mp_tgt mr_tgt1↑)), *)
-        (*     eqr (Any.pair mp_src mr_src1↑) (Any.pair mp_tgt mr_tgt1↑) vret_tgt vret_tgt_tgt) *)
-    :
-      gpaco8 (_sim_itree (mk_wf R) le) (cpn8 (_sim_itree (mk_wf R) le)) r rg _ _ eqr m n a0
-             (Any.pair mp_src mr_src↑, (HoareFunRet Qs mn xs (ctx, vret_src)))
-             (Any.pair mp_tgt mr_tgt↑, (HoareFunRet Qt mn xt (ctx ⋅ rx, vret_tgt)))
-  .
-  Proof.
-    subst. unfold HoareFunRet, mput, mget, guarantee.
-    repeat (ired_both; apply sim_itreeC_spec; econs). exists vret_tgt.
-    steps.
-    repeat (ired_both; apply sim_itreeC_spec; econs).
-    rename c0 into mr_tgt1.
-    assert (exists mr_src1 rret_src,
-               (<<UPDATABLE: URA.wf (ctx ⋅ (mr_tgt1 ⋅ mr_src1 ⋅ rret_src))>>) /\
-               (<<RSRC: R a mp_src mp_tgt mr_src1>>) /\
-               (<<PRE: Qs mn xs vret_src vret_tgt rret_src>>)).
-    { clear - ACC UPDATABLE x0 x1. red in ACC. inv ACC.
-      rename x into vret_tgt_tgt. rename c into rt.
-      specialize (UPDATABLE vret_tgt_tgt).
-      unfold from_iPropL in IPROP.
-      uipropall. des. clarify.
-      rename a1 into rx0.
-      hexploit (UPDATABLE (rt ⋅ rx)); et.
-      { eapply wf_extends; try apply x0. r. exists (ctx ⋅ mr_tgt1). r_solve. }
-      { esplits; eauto. rr in IPROP4. uipropall. eapply IPROP4; eauto.
-        { eapply wf_extends; try apply x0. r. exists (ctx ⋅ mr_tgt1 ⋅ rt). r_solve. }
-        { refl. }
-      }
-      { instantiate (1:=ctx ⋅ mr_tgt1). r_wf x0. }
-      i. des. subst. esplits; [|eauto|eauto].
-      { r_wf H. }
-    }
-    des. exists (rret_src, mr_src1 ⋅ mr_tgt1).
-    steps.
-    repeat (ired_both; apply sim_itreeC_spec; econs). unshelve esplits.
-    { r_wf UPDATABLE0. }
-    repeat (ired_both; apply sim_itreeC_spec; econs). unshelve esplits; eauto.
-    repeat (ired_both; apply sim_itreeC_spec; econs).
-    exploit EQ; et.
-    { econs; et. ii. unfold OwnT. uipropall. esplits; et. refl. }
-    i. uipropall. exploit x3; try apply x1; et.
-    { eapply wf_extends; try apply x0. exists (ctx ⋅ rx ⋅ mr_tgt1). r_solve. }
-    i. rr in x4. uipropall. et.
-  Unshelve. all: ss.
-  Qed.
-
-  Definition HoareCallPre
-             (mn: mname)
-             (tbr: bool)
-             (ord_cur: ord)
-             (fsp: fspec):
-    gname -> Any.t -> Σ -> (itree Es) _ :=
-    fun fn varg_src ctx =>
-      '(rarg, fr, mr) <- trigger (Choose (Σ * Σ * Σ));;
-      _ <- mput mr;;
-      _ <- guarantee(URA.wf (rarg ⋅ fr ⋅ ctx ⋅ mr));;
-
-      x <- trigger (Choose fsp.(meta));; varg_tgt <- trigger (Choose Any.t);;
-      let ord_next := measure fsp x in
-      _ <- guarantee(fsp.(precond) (Some mn) x varg_src varg_tgt rarg);;
-
-      _ <- guarantee(ord_lt ord_next ord_cur /\ (tbr = true -> is_pure ord_next) /\ (tbr = false -> ord_next = ord_top));;
-      Ret (x, fr, varg_tgt)
-  .
-
-  Definition HoareCallPost
-             X
-             (mn: mname)
-             (tbr: bool)
-             (ord_cur: ord)
-             (Q: option string → X → Any.t → Any.t → Σ → Prop)
-             (vret_tgt: Any.t)
-             (x: X)
-             (fr: Σ):
-    itree Es (Σ * Any.t) :=
-      '(rret, ctx) <- trigger (Take (Σ * Σ));;
-      mr <- mget;;
-      _ <- assume(URA.wf (rret ⋅ fr ⋅ ctx ⋅ mr));;
-
-      vret_src <- trigger (Take Any.t);;
-      _ <- assume(Q (Some mn) x vret_src vret_tgt rret);;
-
-      Ret (ctx, vret_src) (*** return to body ***)
-  .
-
-  Lemma HoareCall_parse
-        (mn: mname)
-        (tbr: bool)
-        (ord_cur: ord)
-        (fsp: fspec)
-        (fn: gname)
-        (varg_src: Any.t)
-        (ctx: Σ):
-      HoareCall mn tbr ord_cur fsp fn varg_src ctx =
-      '(x, fr, varg_tgt) <- HoareCallPre mn tbr ord_cur fsp fn varg_src ctx;;
-      vret_tgt <- trigger (Call fn varg_tgt);;
-      HoareCallPost mn tbr ord_cur fsp.(postcond) vret_tgt x fr
-  .
-  Proof.
-    unfold HoareCall, HoareCallPre, HoareCallPost. grind.
-  Qed.
-
-  Lemma hcall_clo_ord_weaken'
-        fsp_src (x_src: shelve__ fsp_src.(meta))
-        fsp_tgt
-
-        A (a0: shelve__ A) FR
-
-        (le: A -> A -> Prop) mn r rg _a n m mp_src0 mp_tgt0 (mr_src0 mr_tgt0: Σ)
-        k_tgt k_src
-        fn tbr_src tbr_tgt ord_cur_src ord_cur_tgt varg_src varg_tgt
-        (R: A -> Any.t -> Any.t -> iProp)
-        (eqr: Any.t -> Any.t -> Any.t -> Any.t -> Prop)
-
-
-        ctx0 rx
-        Invtn Xn Xtra
-        (ACC: current_iPropL ctx0 [(Invtn, OwnT mr_tgt0); (Xn, (Exactly rx Xtra)%I)])
-
-        (UPDATABLE: forall x_tgt,
-           bi_entails (Xtra ** (fsp_tgt.(precond) (Some mn) x_tgt varg_tgt varg_tgt: iProp) **
-                            ⌜ord_lt (measure fsp_tgt x_tgt) ord_cur_tgt
-                             ∧ (tbr_tgt = true → is_pure (measure fsp_tgt x_tgt))
-                             ∧ (tbr_tgt = false → measure fsp_tgt x_tgt = ord_top)⌝)
-                      (bupd (FR ** R a0 mp_src0 mp_tgt0 **
-                                (fsp_src.(precond) (Some mn) x_src varg_src varg_tgt: iProp) **
-                                ⌜ord_lt (measure fsp_src x_src) ord_cur_src
-                             ∧ (tbr_src = true → is_pure (measure fsp_src x_src))
-                             ∧ (tbr_src = false → measure fsp_src x_src = ord_top)⌝
-        )))
-
-        (SIMPLE: forall x_tgt varg_tgt_tgt,
-            (bi_entails ((precond fsp_tgt (Some mn) x_tgt varg_tgt varg_tgt_tgt): iProp) (⌜varg_tgt = varg_tgt_tgt⌝%I)))
-
-        (POST: forall (vret_tgt : Any.t) (mr_src1 mr_tgt1: Σ) (mp_src1 mp_tgt1 : Any.t) a1
-                      (vret_src: Any.t)
-                      (WLE: le a0 a1)
-                      ctx1 fr_tgt x_tgt
-                      (* (ACC: current_iProp ctx1 (FR ** OwnT fr_tgt ** OwnT mr_tgt1 *)
-                      (*                              ** R a1 mp_src1 mp_tgt1 ** fsp_src.(postcond) (Some mn) x_src vret_src vret_tgt)) *)
-                      (ACC: current_iPropL ctx1 [("FR", FR); ("FRT", OwnT fr_tgt); ("INV", R a1 mp_src1 mp_tgt1 ** OwnT mr_tgt1);
-                                                ("POST", fsp_src.(postcond) (Some mn) x_src vret_src vret_tgt)])
-          ,
-                gpaco8 (_sim_itree (mk_wf R) le) (cpn8 (_sim_itree (mk_wf R) le)) rg rg _ _ eqr true true _a
-                       (Any.pair mp_src1 mr_src1↑, k_src (ctx1, vret_src))
-                       (Any.pair mp_tgt1 mr_tgt1↑, HoareCallPost mn tbr_tgt ord_cur_tgt fsp_tgt.(postcond) vret_tgt x_tgt fr_tgt >>= k_tgt)
-        )
-    :
-      gpaco8 (_sim_itree (mk_wf R) le) (cpn8 (_sim_itree (mk_wf R) le)) r rg _ _ eqr m n _a
-             (Any.pair mp_src0 mr_src0↑, (HoareCall mn tbr_src ord_cur_src fsp_src fn varg_src) ctx0 >>= k_src)
-             (Any.pair mp_tgt0 mr_tgt0↑, (HoareCall mn tbr_tgt ord_cur_tgt fsp_tgt fn varg_tgt) (ctx0 ⋅ rx) >>= k_tgt)
-  .
-  Proof.
-    subst. rewrite ! HoareCall_parse. unfold HoareCallPre, mput, mget, assume, guarantee.
-    steps.
-    rename c into mr_tgt1. rename c0 into ro_tgt. rename c1 into fr_tgt.
-    assert(x1 = varg_tgt).
-    { exploit SIMPLE; et. intros T. uipropall.
-      exploit (T ro_tgt); et.
-      { eapply wf_extends; try apply x. r. exists (fr_tgt ⋅ ctx0 ⋅ rx ⋅ mr_tgt1). r_solve.  }
-      intro U. rr in U. uipropall.
-    }
-    subst.
-    assert (exists mr_src1 ro_src fr_src,
-               (<<UPDATABLE: URA.wf (ctx0 ⋅ (mr_tgt1 ⋅ mr_src1 ⋅ ro_src ⋅ fr_src ⋅ fr_tgt))>>) /\
-               (<<RSRC: R a0 mp_src0 mp_tgt0 mr_src1>>) /\
-               (<<FRS: FR fr_src>>) /\
-               (<<PRE: fsp_src.(precond) (Some mn) x_src varg_src varg_tgt ro_src>>) ∧
-               (<<MEASURE: ord_lt (measure fsp_src x_src) ord_cur_src ∧
-                           (tbr_src = true → is_pure (measure fsp_src x_src)) ∧
-                           (tbr_src = false → measure fsp_src x_src = ord_top)>>)
-           ).
-    { clear - ACC UPDATABLE x x0 x2 x3.
-      eapply current_iPropL_pop in ACC; des.
-      eapply current_iPropL_pop in TL; des.
-      eapply current_iPropL_nil in TL0. ss.
-      specialize (UPDATABLE x0).
-      rr in HD0. autorewrite with iprop in HD0. des; clarify. r in HD1. autorewrite with iprop in HD1. des; clarify.
-      uipropall. exploit UPDATABLE; swap 1 2.
-      { esplits; et.
-        { rr in HD1. uipropall. eapply HD1; [|refl].
-          eapply wf_extends; try apply x.
-          exists (ro_tgt ⋅ fr_tgt ⋅ ctx0 ⋅ mr_tgt1). r_solve.
-        }
-        { rr. uipropall. }
-      }
-      { eapply wf_extends; et. r. exists (fr_tgt ⋅ ctx0 ⋅ mr_tgt1). instantiate (1:=ε). r_solve. }
-      { instantiate (1:= fr_tgt ⋅ ctx0 ⋅ mr_tgt1). r_wf x. }
-      i; des. clarify.
-      rr in x8. uipropall. des; ss.
-      esplits; et.
-      { eapply wf_extends; et. r. exists b. r_solve. }
-    }
-    des. (ired_both; apply sim_itreeC_spec; econs).
-    exists (ro_src, fr_src ⋅ fr_tgt, mr_src1 ⋅ mr_tgt1).
-    steps.
-    (ired_both; apply sim_itreeC_spec; econs). unshelve esplits; eauto.
-    { r_wf UPDATABLE0. }
-    (ired_both; apply sim_itreeC_spec; econs). unshelve esplits; eauto.
-    (ired_both; apply sim_itreeC_spec; econs). esplits.
-    (ired_both; apply sim_itreeC_spec; econs). unshelve esplits; eauto.
-    (ired_both; apply sim_itreeC_spec; econs). unshelve esplits; eauto.
-    ired_both. gstep. econs; eauto.
-    { econs; et. i. unfold OwnT. uipropall. esplits; eauto. refl. }
-    i. inv WF.
-
-    unfold HoareCallPost at 1. unfold mget. steps.
-    eapply POST; et.
-    { eapply current_iPropL_push; et.
-      eapply current_iPropL_push; et; cycle 1.
-      { rr. uipropall. refl. }
-      eapply current_iPropL_push; et; cycle 1.
-      { cbn. eapply RSRC0; et. eapply wf_extends; et. exists (c ⋅ fr_src ⋅ fr_tgt ⋅ c0). r_solve. }
-      eapply current_iPropL_push; et; cycle 1.
-      eapply current_iPropL_nil; et.
-      r_wf _ASSUME.
-    }
-  Unshelve. all: ss.
-  Qed.
-
-  Lemma hcall_clo_ord_weaken''
-        fsp_src (x_src: shelve__ fsp_src.(meta))
-        A (a0: shelve__ A) FR
-        fsp_tgt
-
-
-        (le: A -> A -> Prop) mn r rg _a n m mp_src0 mp_tgt0 (mr_src0 mr_tgt0: Σ)
-        k_tgt k_src
-        fn tbr_src tbr_tgt ord_cur_src ord_cur_tgt varg_src varg_tgt
-        (R: A -> Any.t -> Any.t -> iProp)
-        (eqr: Any.t -> Any.t -> Any.t -> Any.t -> Prop)
-
-
-        ctx0 rx
-        ips Xtra
-        (ACC: current_iPropL ctx0 ips)
-        (ENTAIL: bi_entails (from_iPropL ips) (bupd ((OwnT mr_tgt0) ** (Exactly rx Xtra))))
-
-        (UPDATABLE: forall x_tgt,
-           bi_entails (Xtra ** (fsp_tgt.(precond) (Some mn) x_tgt varg_tgt varg_tgt: iProp) **
-                            ⌜ord_lt (measure fsp_tgt x_tgt) ord_cur_tgt
-                             ∧ (tbr_tgt = true → is_pure (measure fsp_tgt x_tgt))
-                             ∧ (tbr_tgt = false → measure fsp_tgt x_tgt = ord_top)⌝
-                      )
-                      (bupd (FR ** R a0 mp_src0 mp_tgt0 ** (fsp_src.(precond) (Some mn) x_src varg_src varg_tgt: iProp)
-                                ** ⌜ord_lt (measure fsp_src x_src) ord_cur_src
-                             ∧ (tbr_src = true → is_pure (measure fsp_src x_src))
-                             ∧ (tbr_src = false → measure fsp_src x_src = ord_top)⌝)))
-
-
-        (SIMPLE: forall x_tgt varg_tgt_tgt,
-            (bi_entails ((precond fsp_tgt (Some mn) x_tgt varg_tgt varg_tgt_tgt): iProp) (⌜varg_tgt = varg_tgt_tgt⌝%I)))
-
-        (POST: forall (vret_tgt : Any.t) (mr_src1 mr_tgt1: Σ) (mp_src1 mp_tgt1 : Any.t) a1
-                      (vret_src: Any.t)
-                      (WLE: le a0 a1)
-                      ctx1 fr_tgt x_tgt
-                      (* (ACC: current_iProp ctx1 (FR ** OwnT fr_tgt ** OwnT mr_tgt1 *)
-                      (*                              ** R a1 mp_src1 mp_tgt1 ** fsp_src.(postcond) (Some mn) x_src vret_src vret_tgt)) *)
-                      (ACC: current_iPropL ctx1 [("FR", FR); ("FRT", OwnT fr_tgt); ("INV", R a1 mp_src1 mp_tgt1 ** OwnT mr_tgt1);
-                                                ("POST", fsp_src.(postcond) (Some mn) x_src vret_src vret_tgt)])
-          ,
-                gpaco8 (_sim_itree (mk_wf R) le) (cpn8 (_sim_itree (mk_wf R) le)) rg rg _ _ eqr true true _a
-                       (Any.pair mp_src1 mr_src1↑, k_src (ctx1, vret_src))
-                       (Any.pair mp_tgt1 mr_tgt1↑, HoareCallPost mn tbr_tgt ord_cur_tgt fsp_tgt.(postcond) vret_tgt x_tgt fr_tgt >>= k_tgt)
-        )
-    :
-      gpaco8 (_sim_itree (mk_wf R) le) (cpn8 (_sim_itree (mk_wf R) le)) r rg _ _ eqr m n _a
-             (Any.pair mp_src0 mr_src0↑, (HoareCall mn tbr_src ord_cur_src fsp_src fn varg_src) ctx0 >>= k_src)
-             (Any.pair mp_tgt0 mr_tgt0↑, (HoareCall mn tbr_tgt ord_cur_tgt fsp_tgt fn varg_tgt) (ctx0 ⋅ rx) >>= k_tgt)
-  .
-  Proof.
-    eapply current_iPropL_entail_all with (Hn:="A") in ACC; et.
-    mDesAll.
-    mAssert _ with "A1". { iAssumption. }
-    mAssert _ with "A". { iAssumption. }
-    eapply hcall_clo_ord_weaken'; et.
-  Qed.
-
-  Lemma hpost_clo_tgt
-        A Xn Xtra Rn Frn Invtn mp_tgt mr_tgt
-        mn r rg
-        Invtn' Xn'
-        X (Q: option mname -> X -> Any.t -> Any.t -> iProp)
-        mpr_src f_src k_tgt
-        a (le: A -> A -> Prop)
-        (R: A -> Any.t -> Any.t -> iProp)
-        (eqr: Any.t -> Any.t -> Any.t -> Any.t -> Prop)
-        m n
-        ctx x vret_tgt vret_src fr_tgt
-        (ACC: current_iPropL ctx [(Rn, Q (Some mn) x vret_src vret_tgt); (Frn, OwnT fr_tgt); (Invtn, OwnT mr_tgt); (Xn, Xtra)])
-        (ARG: forall
-            rx
-            (ACC: current_iPropL ctx [(Invtn', OwnT mr_tgt); (Xn', (Exactly rx Xtra)%I)]),
-            gpaco8 (_sim_itree (mk_wf R) le) (cpn8 (_sim_itree (mk_wf R) le)) r rg _ _ eqr m true a
-                   (mpr_src, f_src)
-                   (Any.pair mp_tgt mr_tgt↑, k_tgt (ctx ⋅ rx, vret_src)))
-        tbr ord_tgt
-    :
-      gpaco8 (_sim_itree (mk_wf R) le) (cpn8 (_sim_itree (mk_wf R) le)) r rg _ _ eqr m n a
-             (mpr_src, f_src)
-             (Any.pair mp_tgt mr_tgt↑, (HoareCallPost mn tbr ord_tgt Q vret_tgt x fr_tgt >>= k_tgt))
-  .
-  Proof.
-    (* inv WF. *)
-    unfold HoareCallPost, mput, mget, assume, guarantee. steps.
-    eapply current_iPropL_pop in ACC. des.
-    eapply current_iPropL_pop in TL. des.
-    eapply current_iPropL_pop in TL0. des.
-    eapply current_iPropL_pop in TL. des. ss. clear_fast.
-    eapply current_iPropL_nil in TL0. rename hdr into rret. rename hdr1 into rinv. rename hdr0 into rf. rename hdr2 into rx.
-    (* apply Any.pair_inj in H2. des; clarify. apply Any.upcast_inj in H0. des; clarify. *)
-    repeat (ired_both; apply sim_itreeC_spec; econs). exists (rret, (ctx ⋅ rx)).
-    repeat (ired_both; apply sim_itreeC_spec; econs). esplits.
-    { clear - TL0 HD1 HD0. unfold OwnT in *. uipropall. unfold URA.extends in *. des; clarify.
-      eapply wf_extends; et. exists (ctx0 ⋅ ctx1). r_solve. }
-    steps.
-    repeat (ired_both; apply sim_itreeC_spec; econs). eexists.
-    repeat (ired_both; apply sim_itreeC_spec; econs). eexists; et. steps.
-    eapply ARG.
-    eapply current_iPropL_push; et.
-    eapply current_iPropL_push; et.
-    { instantiate (1:=rx). eapply current_iPropL_nil; et.
-      { eapply wf_extends; et. exists (rret ⋅ rf). r_solve. }
-    }
-    { rr. uipropall. splits.
-      { refl. }
-      { rr. uipropall. i. eapply iProp_mono; eauto. }
-    }
-  Unshelve. all: try exact 0.
-  Qed.
-
-  Lemma hpost_clo_tgt'
-        A Xn Invtn Xtra mp_tgt mr_tgt
-        mn r rg
-        X (Q: option mname -> X -> Any.t -> Any.t -> iProp)
-        mpr_src f_src k_tgt
-        a (le: A -> A -> Prop)
-        (R: A -> Any.t -> Any.t -> iProp)
-        (eqr: Any.t -> Any.t -> Any.t -> Any.t -> Prop)
-        m n
-        ctx x vret_tgt vret_src fr_tgt ips
-        (ACC: current_iPropL ctx ips)
-        (ENTAIL: bi_entails (from_iPropL ips) (bupd (Q (Some mn) x vret_src vret_tgt ** OwnT fr_tgt ** OwnT mr_tgt ** Xtra)))
-        (ARG: forall
-            rx
-            (ACC: current_iPropL ctx [(Invtn, OwnT mr_tgt); (Xn, (Exactly rx Xtra)%I)]),
-            gpaco8 (_sim_itree (mk_wf R) le) (cpn8 (_sim_itree (mk_wf R) le)) r rg _ _ eqr m true a
-                   (mpr_src, f_src)
-                   (Any.pair mp_tgt mr_tgt↑, k_tgt (ctx ⋅ rx, vret_src)))
-        tbr ord_tgt
-    :
-      gpaco8 (_sim_itree (mk_wf R) le) (cpn8 (_sim_itree (mk_wf R) le)) r rg _ _ eqr m n a
-             (mpr_src, f_src)
-             (Any.pair mp_tgt mr_tgt↑, (HoareCallPost mn tbr ord_tgt Q vret_tgt x fr_tgt >>= k_tgt))
-  .
-  Proof.
-    eapply current_iPropL_entail_all with (Hn:="A") in ACC; et.
-    mDesAll.
-    mAssert _ with "A1". { iAssumption. }
-    mAssert _ with "A2". { iAssumption. }
-    mAssert _ with "A3". { iAssumption. }
-    mAssert _ with "A". { iAssumption. }
-    eapply hpost_clo_tgt; et.
-  Unshelve. all: try exact 0.
-  Qed.
-
   Local Transparent APC.
 
   Definition is_possibly_pure (fsp: fspec): Prop := exists x, is_pure (fsp.(measure) x).
@@ -979,227 +425,158 @@ Section MODE.
 
   Local Transparent HoareCall.
 
-  Lemma hAPC_both
-        A (a0: shelve__ A) mp_src0 mp_tgt0 (mr_src0 mr_tgt0: Σ)
-        mn r rg
-        k_src k_tgt
-        _a (le: A -> A -> Prop)
-        (R: A -> Any.t -> Any.t -> iProp)
-        (eqr: Any.t -> Any.t -> Any.t -> Any.t -> Prop)
-        m n
-        ctx0
-        `{PreOrder _ le}
+  (* Lemma hAPC_both *)
+  (*       A (a0: shelve__ A) mp_src0 mp_tgt0 (mr_src0 mr_tgt0: Σ) *)
+  (*       mn r rg *)
+  (*       k_src k_tgt *)
+  (*       _a (le: A -> A -> Prop) *)
+  (*       (R: A -> Any.t -> Any.t -> iProp) *)
+  (*       (eqr: Any.t -> Any.t -> Any.t -> Any.t -> Prop) *)
+  (*       m n *)
+  (*       ctx0 *)
+  (*       `{PreOrder _ le} *)
 
-        (* (WF: mk_wf R a0 ((Any.pair mp_src0 mr_src0↑), (Any.pair mp_tgt0 mr_tgt0↑))) *)
+  (*       (* (WF: mk_wf R a0 ((Any.pair mp_src0 mr_src0↑), (Any.pair mp_tgt0 mr_tgt0↑))) *) *)
 
-        rx0
-        (* ips Xtra *)
-        (* (ACC: current_iPropL ctx0 ips) *)
-        (* (ENTAIL: bi_entails (from_iPropL ips) ((OwnT mr_tgt0) ** (Xtra ∧ Exactly rx))) *)
-        Xn Invtn Xtra
-        (ACC: current_iPropL ctx0 [(Invtn, OwnT mr_tgt0); (Xn, (Exactly rx0 Xtra)%I)])
-        FR
-        (ENTAIL: bi_entails Xtra (R a0 mp_src0 mp_tgt0 ** FR))
-        (* (WFA: forall a1 mp_src1 mp_tgt1 (mr_src1 mr_tgt1: Σ) (INV: I mr_src1), *)
-        (*     mk_wf R a1 ((Any.pair mp_src1 mr_src1↑), (Any.pair mp_tgt1 mr_tgt1↑))) *)
+  (*       rx0 *)
+  (*       (* ips Xtra *) *)
+  (*       (* (ACC: current_iPropL ctx0 ips) *) *)
+  (*       (* (ENTAIL: bi_entails (from_iPropL ips) ((OwnT mr_tgt0) ** (Xtra ∧ Exactly rx))) *) *)
+  (*       Xn Invtn Xtra *)
+  (*       (ACC: current_iPropL ctx0 [(Invtn, OwnT mr_tgt0); (Xn, (Exactly rx0 Xtra)%I)]) *)
+  (*       FR *)
+  (*       (ENTAIL: bi_entails Xtra (R a0 mp_src0 mp_tgt0 ** FR)) *)
+  (*       (* (WFA: forall a1 mp_src1 mp_tgt1 (mr_src1 mr_tgt1: Σ) (INV: I mr_src1), *) *)
+  (*       (*     mk_wf R a1 ((Any.pair mp_src1 mr_src1↑), (Any.pair mp_tgt1 mr_tgt1↑))) *) *)
 
 
-        stb_src stb_tgt d
-        (STBINCL: stb_pure_incl stb_tgt stb_src)
-        (ARG: forall
-            (mr_src1 mr_tgt1: Σ) (mp_src1 mp_tgt1 : Any.t) a1
-            (WLE: le a0 a1)
-            ctx1 rx1
-            (ACC: current_iPropL ctx1 [("INVT", OwnT mr_tgt1);
-                                      ("X", (Exactly rx1 (R a1 mp_src1 mp_tgt1 ** FR))%I)]),
-            gpaco8 (_sim_itree (mk_wf R) le) (cpn8 (_sim_itree (mk_wf R) le)) rg rg _ _ eqr true true _a
-                   (Any.pair mp_src1 mr_src1↑, k_src (ctx1, tt))
-                   (Any.pair mp_tgt1 mr_tgt1↑, k_tgt (ctx1 ⋅ rx1, tt)))
-    :
-      gpaco8 (_sim_itree (mk_wf R) le) (cpn8 (_sim_itree (mk_wf R) le)) r rg _ _ eqr m n _a
-             (Any.pair mp_src0 mr_src0↑, (interp_hCallE_tgt mn stb_src d APC ctx0) >>= k_src)
-             (Any.pair mp_tgt0 mr_tgt0↑, (interp_hCallE_tgt mn stb_tgt d APC (ctx0 ⋅ rx0)) >>= k_tgt)
-  .
-  Proof.
-    subst.
-    unfold APC. steps. force_l. exists x. steps.
-    deflag.
-    (* Unset Printing Notations. *)
-    clear_until x. gen x d ctx0 rx0. gen mp_src0 mp_tgt0 mr_src0 mr_tgt0. gen a0. gen Xtra. gcofix CIH. i.
-    {
-      rewrite unfold_APC. ired_both.
-      force_r. i. force_l. exists x0.
-      destruct x0.
-      - steps. eapply gpaco8_mon; et.
-        { eapply ARG.
-          { refl. }
-          clear - ACC ENTAIL.
-          eapply current_iPropL_pop in ACC; des.
-          eapply current_iPropL_pop in TL; des.
-          eapply current_iPropL_nil in TL0. ss.
-          eapply current_iPropL_push; et.
-          uipropall. des. clarify.
-          exploit ENTAIL; try apply HD0.
-          { eapply wf_extends; et. r. exists (ctx0 ⋅ hdr). instantiate (1:=hdr0).  r_solve. }
-          { rr in HD1. uipropall. eapply HD1.
-            { eapply wf_extends; [eapply TL0|]. exists (ctx0 ⋅ hdr). r_solve. }
-            { auto. }
-          }            
-          i; des. clarify.
-          eapply current_iPropL_push; cycle 1.
-          { ss. instantiate (1:=a ⋅ b). splits; auto.
-            rr. uipropall. i. eapply ENTAIL; auto.
-            rr in HD1. uipropall. eapply HD1; eauto.
-          }
-          eapply current_iPropL_nil.
-          { r_wf TL0. }
-        }
-      -
-        assert(T: exists rf_src rm_src, R a0 mp_src0 mp_tgt0 rm_src /\ FR rf_src /\ rx0 = rf_src ⋅ rm_src).
-        { clear - ACC ENTAIL. uipropall.
-          eapply current_iPropL_pop in ACC. des.
-          eapply current_iPropL_pop in TL. des.
-          eapply current_iPropL_nil in TL0. ss.
-          des. clarify.
-          exploit ENTAIL; try apply HD0.
-          { eapply wf_extends; et. exists (ctx0 ⋅ hdr). instantiate (1:=hdr0). r_solve. }
-          { rr in HD1. uipropall. eapply HD1.
-            { eapply wf_extends; [eapply TL0|]. exists (ctx0 ⋅ hdr). r_solve. }
-            { auto. }
-          }            
-          i; des. clarify. hexploit (ENTAIL rx0).
-          { eapply wf_extends; eauto. etrans ;eauto.
-            exists (ctx0 ⋅ hdr). r_solve.
-          }
-          { rr in HD1. uipropall. eapply HD1; [|refl].
-            { eapply wf_extends; eauto. etrans ;eauto.
-              exists (ctx0 ⋅ hdr). r_solve.
-            }
-          }
-          { i. des. subst. esplits; eauto. r_solve. }
-        }
-        des. subst.
+  (*       stb_src stb_tgt d *)
+  (*       (STBINCL: stb_pure_incl stb_tgt stb_src) *)
+  (*       (ARG: forall *)
+  (*           (mr_src1 mr_tgt1: Σ) (mp_src1 mp_tgt1 : Any.t) a1 *)
+  (*           (WLE: le a0 a1) *)
+  (*           ctx1 rx1 *)
+  (*           (ACC: current_iPropL ctx1 [("INVT", OwnT mr_tgt1); *)
+  (*                                     ("X", (Exactly rx1 (R a1 mp_src1 mp_tgt1 ** FR))%I)]), *)
+  (*           gpaco8 (_sim_itree (mk_wf R) le) (cpn8 (_sim_itree (mk_wf R) le)) rg rg _ _ eqr true true _a *)
+  (*                  (Any.pair mp_src1 mr_src1↑, k_src (ctx1, tt)) *)
+  (*                  (Any.pair mp_tgt1 mr_tgt1↑, k_tgt (ctx1 ⋅ rx1, tt))) *)
+  (*   : *)
+  (*     gpaco8 (_sim_itree (mk_wf R) le) (cpn8 (_sim_itree (mk_wf R) le)) r rg _ _ eqr m n _a *)
+  (*            (Any.pair mp_src0 mr_src0↑, (interp_hCallE_tgt mn stb_src d APC ctx0) >>= k_src) *)
+  (*            (Any.pair mp_tgt0 mr_tgt0↑, (interp_hCallE_tgt mn stb_tgt d APC (ctx0 ⋅ rx0)) >>= k_tgt) *)
+  (* . *)
+  (* Proof. *)
+  (*   subst. *)
+  (*   unfold APC. steps. force_l. exists x. steps. *)
+  (*   deflag. *)
+  (*   (* Unset Printing Notations. *) *)
+  (*   clear_until x. gen x d ctx0 rx0. gen mp_src0 mp_tgt0 mr_src0 mr_tgt0. gen a0. gen Xtra. gcofix CIH. i. *)
+  (*   { *)
+  (*     rewrite unfold_APC. ired_both. *)
+  (*     force_r. i. force_l. exists x0. *)
+  (*     destruct x0. *)
+  (*     - steps. eapply gpaco8_mon; et. *)
+  (*       { eapply ARG. *)
+  (*         { refl. } *)
+  (*         clear - ACC ENTAIL. *)
+  (*         eapply current_iPropL_pop in ACC; des. *)
+  (*         eapply current_iPropL_pop in TL; des. *)
+  (*         eapply current_iPropL_nil in TL0. ss. *)
+  (*         eapply current_iPropL_push; et. *)
+  (*         uipropall. des. clarify. *)
+  (*         exploit ENTAIL; try apply HD0. *)
+  (*         { eapply wf_extends; et. r. exists (ctx0 ⋅ hdr). instantiate (1:=hdr0).  r_solve. } *)
+  (*         { rr in HD1. uipropall. eapply HD1. *)
+  (*           { eapply wf_extends; [eapply TL0|]. exists (ctx0 ⋅ hdr). r_solve. } *)
+  (*           { auto. } *)
+  (*         }             *)
+  (*         i; des. clarify. *)
+  (*         eapply current_iPropL_push; cycle 1. *)
+  (*         { ss. instantiate (1:=a ⋅ b). splits; auto. *)
+  (*           rr. uipropall. i. eapply ENTAIL; auto. *)
+  (*           rr in HD1. uipropall. eapply HD1; eauto. *)
+  (*         } *)
+  (*         eapply current_iPropL_nil. *)
+  (*         { r_wf TL0. } *)
+  (*       } *)
+  (*     - *)
+  (*       assert(T: exists rf_src rm_src, R a0 mp_src0 mp_tgt0 rm_src /\ FR rf_src /\ rx0 = rf_src ⋅ rm_src). *)
+  (*       { clear - ACC ENTAIL. uipropall. *)
+  (*         eapply current_iPropL_pop in ACC. des. *)
+  (*         eapply current_iPropL_pop in TL. des. *)
+  (*         eapply current_iPropL_nil in TL0. ss. *)
+  (*         des. clarify. *)
+  (*         exploit ENTAIL; try apply HD0. *)
+  (*         { eapply wf_extends; et. exists (ctx0 ⋅ hdr). instantiate (1:=hdr0). r_solve. } *)
+  (*         { rr in HD1. uipropall. eapply HD1. *)
+  (*           { eapply wf_extends; [eapply TL0|]. exists (ctx0 ⋅ hdr). r_solve. } *)
+  (*           { auto. } *)
+  (*         }             *)
+  (*         i; des. clarify. hexploit (ENTAIL rx0). *)
+  (*         { eapply wf_extends; eauto. etrans ;eauto. *)
+  (*           exists (ctx0 ⋅ hdr). r_solve. *)
+  (*         } *)
+  (*         { rr in HD1. uipropall. eapply HD1; [|refl]. *)
+  (*           { eapply wf_extends; eauto. etrans ;eauto. *)
+  (*             exists (ctx0 ⋅ hdr). r_solve. *)
+  (*           } *)
+  (*         } *)
+  (*         { i. des. subst. esplits; eauto. r_solve. } *)
+  (*       } *)
+  (*       des. subst. *)
 
-        steps. force_l. exists x0. steps. force_l; ss. steps. unfold HoareCall. unfold mput, mget. steps.
-        des; ss.
-        assert(STB: stb_src s = Some f).
-        { eapply STBINCL; et. r. esplits; et. }
-        force_l. eexists (_, _). steps. rewrite STB. steps. instantiate (1:=t).
-        unfold HoareCall. unfold mput, mget. steps.
+  (*       steps. force_l. exists x0. steps. force_l; ss. steps. unfold HoareCall. unfold mput, mget. steps. *)
+  (*       des; ss. *)
+  (*       assert(STB: stb_src s = Some f). *)
+  (*       { eapply STBINCL; et. r. esplits; et. } *)
+  (*       force_l. eexists (_, _). steps. rewrite STB. steps. instantiate (1:=t). *)
+  (*       unfold HoareCall. unfold mput, mget. steps. *)
 
-        force_l. rename c into mr_tgt1. rename c0 into ro. rename c1 into rf.
-        exists (ro, rf ⋅ rf_src, rm_src ⋅ mr_tgt1). steps. force_l; ss.
-        { r_wf _GUARANTEE1. }
-        steps. force_l. esplits; et. steps. force_l. esplits; et. steps. force_l. esplits; et.
-        steps. force_l; et. steps. gstep. econs; eauto.
-        { econs. eapply to_semantic. iIntros "[A B]". iFrame. iStopProof.
-          uipropall. i. eapply iProp_mono; et.
-        }
+  (*       force_l. rename c into mr_tgt1. rename c0 into ro. rename c1 into rf. *)
+  (*       exists (ro, rf ⋅ rf_src, rm_src ⋅ mr_tgt1). steps. force_l; ss. *)
+  (*       { r_wf _GUARANTEE1. } *)
+  (*       steps. force_l. esplits; et. steps. force_l. esplits; et. steps. force_l. esplits; et. *)
+  (*       steps. force_l; et. steps. gstep. econs; eauto. *)
+  (*       { econs. eapply to_semantic. iIntros "[A B]". iFrame. iStopProof. *)
+  (*         uipropall. i. eapply iProp_mono; et. *)
+  (*       } *)
 
-        i. inv WF. clarify. steps.
-        hexploit1 RSRC.
-        { eapply wf_extends; et. r. exists (c ⋅ rf ⋅ rf_src ⋅ c0). r_solve. }
-        rename c into ri. rename c0 into ctx1.
-        rr in RSRC. autounfold with iprop in RSRC; autorewrite with iprop in RSRC. des. clarify.
-        rename a into rinv.
-        force_r. exists (ri, ctx1 ⋅ (rinv ⋅ rf_src)). steps. force_r; ss.
-        { rr in RSRC1. uipropall. red in RSRC1. des. subst.
-          eapply wf_extends; eauto. exists ctx. r_solve.
-        }
-        steps. force_r. esplits. steps. force_r; et. steps.
+  (*       i. inv WF. clarify. steps. *)
+  (*       hexploit1 RSRC. *)
+  (*       { eapply wf_extends; et. r. exists (c ⋅ rf ⋅ rf_src ⋅ c0). r_solve. } *)
+  (*       rename c into ri. rename c0 into ctx1. *)
+  (*       rr in RSRC. autounfold with iprop in RSRC; autorewrite with iprop in RSRC. des. clarify. *)
+  (*       rename a into rinv. *)
+  (*       force_r. exists (ri, ctx1 ⋅ (rinv ⋅ rf_src)). steps. force_r; ss. *)
+  (*       { rr in RSRC1. uipropall. red in RSRC1. des. subst. *)
+  (*         eapply wf_extends; eauto. exists ctx. r_solve. *)
+  (*       } *)
+  (*       steps. force_r. esplits. steps. force_r; et. steps. *)
 
-        move CIH at bottom.
-        deflag. gbase. eapply (CIH _ w1); et.
-        { i. eapply ARG; try apply ACC0. etrans; et. }
-        { eapply current_iPropL_push; et.
-          eapply current_iPropL_push; cycle 1.
-          { ss. rr. uipropall. splits.
-            { refl. }
-            rr. uipropall. i. r in H0. des. subst.
-            exists (rinv ⋅ ctx), rf_src. esplits.
-            { r_solve. }
-            { eapply iProp_mono; [..|eauto]; eauto.
-              { eapply wf_extends; eauto. exists rf_src. r_solve. }
-              { exists ctx. r_solve. }
-            }
-            { eauto. }
-          }
-          eapply current_iPropL_nil.
-          eapply wf_extends; try apply _ASSUME.
-          exists (ri ⋅ rf). r_solve.
-        }
-    }
-  Unshelve. all: try exact 0.
-  Qed.
+  (*       move CIH at bottom. *)
+  (*       deflag. gbase. eapply (CIH _ w1); et. *)
+  (*       { i. eapply ARG; try apply ACC0. etrans; et. } *)
+  (*       { eapply current_iPropL_push; et. *)
+  (*         eapply current_iPropL_push; cycle 1. *)
+  (*         { ss. rr. uipropall. splits. *)
+  (*           { refl. } *)
+  (*           rr. uipropall. i. r in H0. des. subst. *)
+  (*           exists (rinv ⋅ ctx), rf_src. esplits. *)
+  (*           { r_solve. } *)
+  (*           { eapply iProp_mono; [..|eauto]; eauto. *)
+  (*             { eapply wf_extends; eauto. exists rf_src. r_solve. } *)
+  (*             { exists ctx. r_solve. } *)
+  (*           } *)
+  (*           { eauto. } *)
+  (*         } *)
+  (*         eapply current_iPropL_nil. *)
+  (*         eapply wf_extends; try apply _ASSUME. *)
+  (*         exists (ri ⋅ rf). r_solve. *)
+  (*       } *)
+  (*   } *)
+  (* Unshelve. all: try exact 0. *)
+  (* Qed. *)
 
 End MODE.
 
-Global Opaque OwnT.
-
-Ltac harg :=
-  let PRE := constr:("PRE") in
-  let INVS := constr:("INVS") in
-  let INVT := constr:("INVT") in
-  eapply (@harg_clo _ _ PRE INVS INVT);
-  [eassumption
-  |
-  ]; i.
-
-
-
-Ltac init :=
-  let varg_src := fresh "varg_src" in
-  let mn := fresh "mn" in
-  let varg := fresh "varg" in
-  let EQ := fresh "EQ" in
-  let w := fresh "w" in
-  let mrp_src := fresh "mrp_src" in
-  let mp_tgt := fresh "mp_tgt" in
-  let WF := fresh "WF" in
-  split; rr; ss; intros varg_src [mn varg] EQ w mrp_src mp_tgt WF;
-  (try subst varg_src); cbn;
-  ginit;
-  try (unfold fun_to_tgt, cfunN, cfunU; rewrite ! HoareFun_parse); simpl.
-
-Ltac harg_tgt :=
-  let XN := constr:("FR") in
-  let INVTN := constr:("INVT") in
-  eapply (@harg_clo_tgt' _ _ XN INVTN);
-  [eassumption
-  |start_ipm_proof
-  |on_current ltac:(fun H => try clear H); i; on_current ltac:(fun H => simpl in H)].
-
-Ltac hpost_tgt :=
-  let XN := constr:("FR") in
-  let INVTN := constr:("INVT") in
-  eapply (@hpost_clo_tgt' _ _ XN INVTN);
-  [eassumption
-  |start_ipm_proof
-  |on_current ltac:(fun H => try clear H); i; on_current ltac:(fun H => simpl in H)].
-
-Tactic Notation "hcall" uconstr(x) uconstr(a) :=
-  eapply (@hcall_clo_ord_weaken'' _ _ x _ a);
-  unshelve_goal;
-  [eassumption
-  |start_ipm_proof; try (iFrame; et)
-  |cbn; i; iIntros "[FR P]"
-  |
-  |on_current ltac:(fun H => try clear H); i; on_current ltac:(fun H => simpl in H)]
-.
-
-Tactic Notation "hret" uconstr(a) :=
-  eapply (@hret_clo_both _ _ a); unshelve_goal;
-  [eassumption
-  |
-  |i; iIntros "[Q FR]"
-  |i; iIntros "Q"
-  ].
-
-Tactic Notation "hAPC" uconstr(a) :=
-  eapply (@hAPC_both _ _ a);
-  [try (typeclasses eauto)
-  |eassumption
-  |
-  |
-  |on_current ltac:(fun H => try clear H); i; on_current ltac:(fun H => simpl in H)]
-.
